\documentclass{article}

\usepackage{amsmath}
\usepackage{amssymb}

\title{Calculations Pertaining to Analytically Determining Arc Lengths of Gaussian Porcesses}
\author{Nathan Wycoff}


\begin{document}
	\maketitle
	
	\section{Lines as parametric equations}
	
	In higher dimensional spaces, lines need to be expressed as parametric equations.
	
	In particular, the line segment connecting $a$ and $b$ may be expressed as such:
	
	$$f(t) = a + t(b-a), t \in [0,1]$$
	
	It may also be desireable to scale $t$ such that a one unit change in $t$ corresponds to a movement of one unit in euclidean terms in the high D space:
	
	$$f(t) = a + \frac{b - a}{||b - a||_2} t, t \in [0,||b - a||_2]$$
	
	\section{Generalized Arc Length of a GP Mean Surface for General Kernel}
	
    In this section, we will semi-rigorously derive the arc length along a line for $\mathbb{R}^n$ equipped with an p-norm along a GP mean surface, a slight generalization of arc length in Euclidean space, which follows a very similar derivation.
	
    Begin with the limit definition of arc-length from $a$ to $b$, $a,b \in \mathbb{R}^n$. Let $t_i = a + \frac{b-a}{n}i$ (that is, $t_i$ represents some point along the line from $a$ to $b$), and $s(x,y)$ represent the line segment from $x$ to $y$.

    $$\textrm{ArcLen} = \lim_{n\to\infty} \sum_{i=1}^{n} ||s(\mu(t_i), \mu(t_{i-1})||_p$$

    That is, simply the sum of the vanishingly small line segments along the path.

    For p-norms, we can separate the norm as such:

    $$\textrm{ArcLen} = \lim_{n\to\infty} \sum_{i=1}^{n} (||s(t_i,t_{i-1})||_p^p + (|\mu(t_i) - \mu(t_{i-1})|)^p)^{\frac{1}{p}}$$

	and re-arrange the limit:

    $$ = \lim_{n\to\infty} \sum_{i=1}^{n} (||s(t_i,t_{i-1})||_p^p + (|\mu(t_{i-1} + \frac{b-a}{n}) - \mu(t_{i-1})|)^p)^{\frac{1}{p}}$$
    
    $$ = \lim_{n\to\infty} \sum_{i=1}^{n} ((\frac{||b-a||_p}{n})^p + (|\mu(t_{i-1} + 
    \frac{||b-a||_p}{n} \frac{b-a}{||b-a||_p}) - \mu(t_{i-1})|)^p)^{\frac{1}{p}}$$
    	
    $$ =  \lim_{n\to\infty} \sum_{i=1}^{n} ((\frac{||b-a||_p}{n})^p + (|\frac{||b-a||_p}{n} \frac{\mu(t_{i-1} + 
    \frac{||b-a||_p}{n} \frac{b-a}{||b-a||_p}) - \mu(t_{i-1})}{\frac{||b-a||_p}{n}}|)^p)^{\frac{1}{p}}$$

	$$ =  ||b-a||_p\lim_{n\to\infty} \frac{1}{n} \sum_{i=1}^{n} ( 1 + (|\frac{\mu(t_{i-1} + 
		\frac{||b-a||_p}{n} \frac{b-a}{||b-a||_p}) - \mu(t_{i-1})}{\frac{||b-a||_p}{n}}|)^p)^{\frac{1}{p}}$$
	
	 We notice that, $n\to \infty \implies \frac{||b-a||_p}{n} \to 0$, which means that:
	 
	 $$ \lim_{n\to\infty}  \frac{\mu(t_{i-1} + 
	 	\frac{||b-a||_p}{n} \frac{b-a}{||b-a||_p}) - \mu(t_{i-1})}{\frac{||b-a||_p}{n}} = 
 	\lim_{h\to 0}  \frac{\mu(t_{i-1} + 
 		h \frac{b-a}{||b-a||_p}) - \mu(t_{i-1})}{h} $$
 	
 	$ = (\nabla_{b-a} \mu)(t_{i-1})$, the directional derivative of $\mu$ in the direction of $b-a$ evaluated at $t_{i-1}$.
	 
	 Now for the hand-wavy part: speaking very loosely:
	
	$$\lim_{n\to\infty} \frac{1}{n} \sum_{i=1}^n f(t_{i}) - f(t_{i-1}) = \int_{a}^b f(t)dt$$
	
	so we have, in our case:
	
	$$||b-a||_p\lim_{n\to\infty} \frac{1}{n} \sum_{i=1}^{n} ( 1 + (|\frac{\mu(t_{i-1} + 
		\frac{||b-a||_p}{n} \frac{b-a}{||b-a||_p}) - \mu(t_{i-1})}{\frac{||b-a||_p}{n}}|)^p)^{\frac{1}{p}} $$
	
	$$= \int_{0}^{1} (1 + (|\nabla_{b-a} \mu)(a + t(b-a)|)^p)^{1/p} dt$$
	
	, our desired result.
	
\end{document}
